HOL-Light: Autogenerate zeta tables in proof scripts
This commit extends `autogen` to autogenerate the OCaml list
of zeta values used in the HOL-Light specs for the AArch64
forward and inverse NTTs.

This is reusing the same generator for the zeta values that is
already used for the autogeneration of the C zeta tables, but
uses a new formatter for OCaml.

Signed-off-by: Hanno Becker <beckphan@amazon.co.uk>

proofs/hol_light/arm/proofs/mlkem_intt.ml
@@ -11,6 +11,7 @@ needs "arm/proofs/base.ml";;
 
 needs "proofs/mlkem_specs.ml";;
 needs "proofs/mlkem_utils.ml";;
+needs "proofs/mlkem_zetas.ml";;
 
 (**** print_literal_from_elf "mlkem/mlkem_intt.o";;
  ****)
@@ -468,94 +469,28 @@ let mlkem_intt_mc = define_assert_from_elf
 
 let MLKEM_INTT_EXEC = ARM_MK_EXEC_RULE mlkem_intt_mc;;
 
-(* ------------------------------------------------------------------------- *)
-(* Data tables that are assumed in the precondition.                         *)
-(* ------------------------------------------------------------------------- *)
-
-let intt_zetas_layer01234 = define
- `intt_zetas_layer01234:int list =
-   [&1583; &15582; -- &821; -- &8081; &1355; &13338; &0; &0; -- &569; -- &5601;
-    &450; &4429; &936; &9213; &0; &0; &69; &679; &447; &4400; -- &535;
-    -- &5266; &0; &0; &543; &5345; &1235; &12156; -- &1426; -- &14036; &0;
-    &0; -- &797; -- &7845; -- &1333; -- &13121; &1089; &10719; &0; &0;
-    -- &193; -- &1900; -- &56; -- &551; &283; &2786; &0; &0; &1410; &13879;
-    -- &1476; -- &14529; -- &1339; -- &13180; &0; &0; -- &1062; -- &10453;
-    &882; &8682; -- &296; -- &2914; &0; &0; &1600; &15749; &40; &394;
-    &749; &7373; -- &848; -- &8347; &1432; &14095; -- &630; -- &6201;
-    &687; &6762; &0; &0]`;;
-
-let intt_zetas_layer56 = define
- `intt_zetas_layer56:int list =
-   [-- &910; -- &910; -- &1227; -- &1227; &219; &219; &855; &855; -- &8957;
-    -- &8957; -- &12078; -- &12078; &2156; &2156; &8416; &8416; &1175;
-    &1175; &394; &394; -- &1029; -- &1029; -- &1212; -- &1212; &11566;
-    &11566; &3878; &3878; -- &10129; -- &10129; -- &11930; -- &11930;
-    -- &885; -- &885; &1219; &1219; &1455; &1455; &1607; &1607; -- &8711;
-    -- &8711; &11999; &11999; &14322; &14322; &15818; &15818; -- &648;
-    -- &648; -- &1481; -- &1481; &712; &712; &682; &682; -- &6378; -- &6378;
-    -- &14578; -- &14578; &7008; &7008; &6713; &6713; -- &886; -- &886;
-    &1179; &1179; -- &1026; -- &1026; -- &1092; -- &1092; -- &8721;
-    -- &8721; &11605; &11605; -- &10099; -- &10099; -- &10749; -- &10749;
-    &554; &554; -- &1143; -- &1143; -- &403; -- &403; &525; &525; &5453;
-    &5453; -- &11251; -- &11251; -- &3967; -- &3967; &5168; &5168; &927;
-    &927; -- &1534; -- &1534; &461; &461; -- &1438; -- &1438; &9125;
-    &9125; -- &15099; -- &15099; &4538; &4538; -- &14155; -- &14155; &735;
-    &735; -- &561; -- &561; -- &757; -- &757; -- &319; -- &319; &7235;
-    &7235; -- &5522; -- &5522; -- &7451; -- &7451; -- &3140; -- &3140;
-    &863; &863; &1230; &1230; &556; &556; -- &1063; -- &1063; &8495;
-    &8495; &12107; &12107; &5473; &5473; -- &10463; -- &10463; -- &452;
-    -- &452; -- &807; -- &807; -- &1435; -- &1435; &1010; &1010; -- &4449;
-    -- &4449; -- &7943; -- &7943; -- &14125; -- &14125; &9942; &9942;
-    -- &1645; -- &1645; &780; &780; &109; &109; &1031; &1031; -- &16192;
-    -- &16192; &7678; &7678; &1073; &1073; &10148; &10148; &1239; &1239;
-    -- &375; -- &375; &1292; &1292; -- &1584; -- &1584; &12196; &12196;
-    -- &3691; -- &3691; &12717; &12717; -- &15592; -- &15592; &1414; &1414;
-    -- &1320; -- &1320; -- &33; -- &33; &464; &464; &13918; &13918;
-    -- &12993; -- &12993; -- &325; -- &325; &4567; &4567; -- &641; -- &641;
-    &992; &992; &941; &941; &1021; &1021; -- &6309; -- &6309; &9764;
-    &9764; &9262; &9262; &10050; &10050; -- &268; -- &268; -- &733;
-    -- &733; &892; &892; -- &939; -- &939; -- &2638; -- &2638; -- &7215;
-    -- &7215; &8780; &8780; -- &9243; -- &9243; -- &632; -- &632; &816; &816;
-    &1352; &1352; -- &650; -- &650; -- &6221; -- &6221; &8032; &8032;
-    &13308; &13308; -- &6398; -- &6398; &642; &642; -- &952; -- &952;
-    &1540; &1540; -- &1651; -- &1651; &6319; &6319; -- &9371; -- &9371;
-    &15159; &15159; -- &16251; -- &16251; -- &1461; -- &1461; &1482;
-    &1482; &540; &540; &1626; &1626; -- &14381; -- &14381; &14588; &14588;
-    &5315; &5315; &16005; &16005; &1274; &1274; &1052; &1052; &1025;
-    &1025; -- &1197; -- &1197; &12540; &12540; &10355; &10355; &10089;
-    &10089; -- &11782; -- &11782; &279; &279; &1173; &1173; -- &233;
-    -- &233; &667; &667; &2746; &2746; &11546; &11546; -- &2293; -- &2293;
-    &6565; &6565; &314; &314; -- &756; -- &756; &48; &48; -- &1409;
-    -- &1409; &3091; &3091; -- &7441; -- &7441; &472; &472; -- &13869;
-    -- &13869; &1573; &1573; &76; &76; -- &331; -- &331; -- &289; -- &289;
-    &15483; &15483; &748; &748; -- &3258; -- &3258; -- &2845; -- &2845;
-    -- &1100; -- &1100; -- &723; -- &723; &680; &680; &568; &568; -- &10828;
-    -- &10828; -- &7117; -- &7117; &6693; &6693; &5591; &5591; &1041;
-    &1041; -- &1637; -- &1637; -- &583; -- &583; -- &17; -- &17; &10247;
-    &10247; -- &16113; -- &16113; -- &5739; -- &5739; -- &167; -- &167]`;;
-
 let intt_constants = define
- `intt_constants z_01234 z_56 s <=>
+ `intt_constants z_12345 z_67 s <=>
         (!i. i < 80
-             ==> read(memory :> bytes16(word_add z_01234 (word(2 * i)))) s =
-                 iword(EL i intt_zetas_layer01234)) /\
+             ==> read(memory :> bytes16(word_add z_12345 (word(2 * i)))) s =
+                 iword(EL i intt_zetas_layer12345)) /\
         (!i. i < 384
-             ==> read(memory :> bytes16(word_add z_56 (word(2 * i)))) s =
-                 iword(EL i intt_zetas_layer56))`;;
+             ==> read(memory :> bytes16(word_add z_67 (word(2 * i)))) s =
+                 iword(EL i intt_zetas_layer67))`;;
 
 (* ------------------------------------------------------------------------- *)
 (* Correctness proof.                                                        *)
 (* ------------------------------------------------------------------------- *)
 
 let MLKEM_INTT_CORRECT = prove
- (`!a z_01234 z_56 x pc.
+ (`!a z_12345 z_67 x pc.
       ALL (nonoverlapping (a,512))
-          [(word pc,0x6f8); (z_01234,160); (z_56,768)]
+          [(word pc,0x6f8); (z_12345,160); (z_67,768)]
       ==> ensures arm
            (\s. aligned_bytes_loaded s (word pc) mlkem_intt_mc /\
                 read PC s = word (pc + 0x14) /\
-                C_ARGUMENTS [a; z_01234; z_56] s /\
-                intt_constants z_01234 z_56 s /\
+                C_ARGUMENTS [a; z_12345; z_67] s /\
+                intt_constants z_12345 z_67 s /\
                 !i. i < 256
                     ==> read(memory :> bytes16(word_add a (word(2 * i)))) s =
                         x i)
@@ -569,7 +504,7 @@ let MLKEM_INTT_CORRECT = prove
             MAYCHANGE [Q8; Q9; Q10; Q11; Q12; Q13; Q14; Q15] ,,
             MAYCHANGE [memory :> bytes(a,512)])`,
   MAP_EVERY X_GEN_TAC
-   [`a:int64`; `z_01234:int64`; `z_56:int64`; `x:num->int16`; `pc:num`] THEN
+   [`a:int64`; `z_12345:int64`; `z_67:int64`; `x:num->int16`; `pc:num`] THEN
   REWRITE_TAC[MAYCHANGE_REGS_AND_FLAGS_PERMITTED_BY_ABI; C_ARGUMENTS;
               NONOVERLAPPING_CLAUSES; ALL] THEN
   DISCH_THEN(REPEAT_TCL CONJUNCTS_THEN ASSUME_TAC) THEN
@@ -579,7 +514,7 @@ let MLKEM_INTT_CORRECT = prove
   REWRITE_TAC[intt_constants] THEN
   CONV_TAC(RATOR_CONV(LAND_CONV(ONCE_DEPTH_CONV
    (EXPAND_CASES_CONV THENC ONCE_DEPTH_CONV NUM_MULT_CONV)))) THEN
-  REWRITE_TAC[intt_zetas_layer01234; intt_zetas_layer56] THEN
+  REWRITE_TAC[intt_zetas_layer12345; intt_zetas_layer67] THEN
   CONV_TAC(ONCE_DEPTH_CONV EL_CONV) THEN
   CONV_TAC(ONCE_DEPTH_CONV WORD_IWORD_CONV) THEN REWRITE_TAC[WORD_ADD_0] THEN
   ENSURES_INIT_TAC "s0" THEN
@@ -589,8 +524,8 @@ let MLKEM_INTT_CORRECT = prove
    ***)
 
   MEMORY_128_FROM_16_TAC "a" 32 THEN
-  MEMORY_128_FROM_16_TAC "z_01234" 10 THEN
-  MEMORY_128_FROM_16_TAC "z_56" 48 THEN
+  MEMORY_128_FROM_16_TAC "z_12345" 10 THEN
+  MEMORY_128_FROM_16_TAC "z_67" 48 THEN
   ASM_REWRITE_TAC[WORD_ADD_0] THEN CONV_TAC WORD_REDUCE_CONV THEN
   DISCARD_MATCHING_ASSUMPTIONS [`read (memory :> bytes16 a) s = x`] THEN
   REPEAT STRIP_TAC THEN
@@ -641,19 +576,19 @@ let MLKEM_INTT_CORRECT = prove
 (*** Subroutine form, somewhat messy elaboration of the usual wrapper ***)
 
 let MLKEM_INTT_SUBROUTINE_CORRECT = prove
- (`!a z_01234 z_56 x pc stackpointer returnaddress.
+ (`!a z_12345 z_67 x pc stackpointer returnaddress.
       aligned 16 stackpointer /\
       ALLPAIRS nonoverlapping
        [(a,512); (word_sub stackpointer (word 64),64)]
-       [(word pc,0x6f8); (z_01234,160); (z_56,768)] /\
+       [(word pc,0x6f8); (z_12345,160); (z_67,768)] /\
       nonoverlapping (a,512) (word_sub stackpointer (word 64),64)
       ==> ensures arm
            (\s. aligned_bytes_loaded s (word pc) mlkem_intt_mc /\
                 read PC s = word pc /\
                 read SP s = stackpointer /\
                 read X30 s = returnaddress /\
-                C_ARGUMENTS [a; z_01234; z_56] s /\
-                intt_constants z_01234 z_56 s /\
+                C_ARGUMENTS [a; z_12345; z_67] s /\
+                intt_constants z_12345 z_67 s /\
                 !i. i < 256
                     ==> read(memory :> bytes16(word_add a (word(2 * i)))) s =
                         x i)
